wip

LeanSubst/Basic.lean
@@ -1,6 +1,6 @@
 
-import Lean.Elab.Term
-import Lean.Elab.SyntheticMVars
+-- import Lean.Elab.Term
+-- import Lean.Elab.SyntheticMVars
 
 -- import LeanSubst.Glue
 
@@ -17,9 +17,6 @@ infixr:67 (name := «_.:_») " .: " => AltCons.altCons
 
 @[reducible]
 def Subst.typeof {T : Type u2} (_ : T) : Type u2 := T
-
-set_option linter.unusedVariables false in
-abbrev Var (T : Type u2) := Nat
 
 structure Ren (T : Type u2) : Type u2 where
   act : Nat -> Nat
@@ -169,5 +166,286 @@ def unexpand_smap : Lean.PrettyPrinter.Unexpander
 | `($_ ($σ1, $σ2, $σ3, SubstVec.nil) $t) => `($t[$σ1, $σ2, $σ3])
 | `($_ $σ $t) => `($t[$σ,])
 | _ => throw ()
+
+@[reducible, simp]
+instance [i : RenMapAll (T::V)] : RenMap T (T::V) where
+  rmap :=
+    match i with
+    | @RenMapAll.cons _ _ i _ => i.rmap
+
+set_option synthInstance.checkSynthOrder false in
+@[reducible, simp]
+instance [i : RenMapAll (T::V)] : RenMapAll V :=
+  match i with
+  | @RenMapAll.cons _ _ _ i => i
+
+@[reducible, simp]
+instance [i : SubstMapAll (T::V)] : SubstMap T (T::V) where
+  smap :=
+    match i with
+    | @SubstMapAll.cons _ _ i _ => i.smap
+
+set_option synthInstance.checkSynthOrder false in
+@[reducible, simp]
+instance [i : SubstMapAll (T::V)] : SubstMapAll V :=
+  match i with
+  | @SubstMapAll.cons _ _ _ i => i
+
+def RenVec.head : RenVec (T::V) -> Ren T
+| cons r _ => r
+
+def RenVec.tail : RenVec (T::V) -> RenVec V
+| cons _ r => r
+
+@[simp]
+theorem RenVec.head_cons {r : Ren T} {rs : RenVec V} : (r .: rs).head = r := by simp [head]
+
+@[simp]
+theorem RenVec.tail_cons {r : Ren T} {rs : RenVec V} : (r .: rs).tail = rs := by simp [tail]
+
+def SubstVec.head : SubstVec (T::V) -> Subst T
+| cons σ _ => σ
+
+def SubstVec.tail : SubstVec (T::V) -> SubstVec V
+| cons _ σ => σ
+
+@[simp]
+theorem SubstVec.head_cons {σ : Subst T} {σs : SubstVec V} : (σ .: σs).head = σ := by simp [head]
+
+@[simp]
+theorem SubstVec.tail_cons {σ : Subst T} {σs : SubstVec V} : (σ .: σs).tail = σs := by simp [tail]
+
+@[simp]
+theorem Subst.act_inner {f : Nat -> Action T} {x} : Subst.act { inner := f } x = f x := by
+  simp [act, SubstAction.act]
+
+@[simp]
+def Action.rmap1 [RenMap T (T::V)] (r : RenVec (T::V)) : Action T -> Action T
+| re x => re $ r.head.act x
+| su t => su t⟨r,⟩
+
+instance [RenMap T (T::V)] : RenMap (Action T) (T::V) where
+  rmap v := Action.rmap1 v
+
+@[simp]
+theorem Action.rmap1_re [RenMap T (T::V)] {r : RenVec (T::V)} {x : Nat}
+  : (@re T x)⟨r,⟩ = re (r.head.act x)
+:= by simp [RenMap.rmap]
+
+@[simp]
+theorem Action.rmap1_su [RenMap T (T::V)] {r : RenVec (T::V)} {t : T} : (su t)⟨r,⟩ = su t⟨r,⟩ := by
+  simp [RenMap.rmap]
+
+@[simp]
+def Action.rmap0 [RenMap S V] (r : RenVec V) : Action S -> Action S
+| re x => re x
+| su t => su t⟨r,⟩
+
+instance [RenMap S V] [RenSuffix S V] : RenMap (Action S) V where
+  rmap := Action.rmap0
+
+@[simp]
+theorem Action.rmap0_re [RenMap S V] [RenSuffix S V] {r : RenVec V} {x : Nat}
+  : (@re S x)⟨r,⟩ = re x
+:= by simp [RenMap.rmap]
+
+@[simp]
+theorem Action.rmap0_su [RenMap S V] [RenSuffix S V] {r : RenVec V} {t : S}
+  : (su t)⟨r,⟩ = su t⟨r,⟩
+:= by simp [RenMap.rmap]
+
+@[simp]
+def Action.smap1 [SubstMap T (T::V)] (σ : SubstVec (T::V)) : Action T -> Action T
+| re x => σ.head.act x
+| su t => su t[σ,]
+
+instance [SubstMap T (T::V)] : SubstMap (Action T) (T::V) where
+  smap v := Action.smap1 v
+
+@[simp]
+theorem Action.smap1_re [SubstMap T (T::V)] {σ : SubstVec (T::V)} {x : Nat}
+  : (@re T x)[σ,] = σ.head.act x
+:= by simp [SubstMap.smap, Subst.act, SubstAction.act]
+
+@[simp]
+theorem Action.smap1_su [SubstMap T (T::V)] {σ : SubstVec (T::V)} {t : T}
+  : (su t)[σ,] = su t[σ,]
+:= by simp [SubstMap.smap]
+
+@[simp]
+def Action.smap0 [SubstMap S V] (σ : SubstVec V) : Action S -> Action S
+| re x => re x
+| su t => su t[σ,]
+
+instance [SubstMap S V] [SubstSuffix S V] : SubstMap (Action S) V where
+  smap := Action.smap0
+
+@[simp]
+theorem Action.smap0_re [SubstMap S V] [SubstSuffix S V] {σ : SubstVec V} {x : Nat}
+  : (@re S x)[σ,] = re x
+:= by simp [SubstMap.smap]
+
+@[simp]
+theorem Action.smap0_su [SubstMap S V] [SubstSuffix S V] {σ : SubstVec V} {t : S}
+  : (su t)[σ,] = su t[σ,]
+:= by simp [SubstMap.smap]
+
+def Ren.id T : Ren T := ⟨λ x => x⟩
+notation "𝐫0" => Ren.id _
+notation "𝐫0(" T ")" => Ren.id T
+
+@[reducible, simp]
+def RenVec.id : (V : List (Type u2)) -> RenVec V
+| [] => .nil
+| .cons x xs => .id x .: id xs
+
+def Subst.id T : Subst T := ⟨λ x => re x⟩
+notation "𝐬0" => Subst.id _
+notation "𝐬0(" T ")" => Subst.id T
+
+@[reducible, simp]
+def SubstVec.id : (V : List (Type u2)) -> SubstVec V
+| [] => .nil
+| .cons x xs => .id x .: id xs
+
+def Ren.add T (k : Nat) : Ren T := ⟨(· + k)⟩
+
+def Subst.add T (k : Nat) : Subst T := ⟨λ x => re $ x + k⟩
+
+def Ren.sub T (k : Nat) : Ren T := ⟨(· - k)⟩
+
+def Subst.sub T (k : Nat) : Subst T := ⟨λ x => re $ x - k⟩
+
+def Ren.cons (a : Nat) (r : Ren T) : Ren T := .mk λ n =>
+  match n with
+  | 0 => a
+  | n + 1 => r.act n
+
+instance : AltCons Nat (Ren T) where
+  altCons := Ren.cons
+
+def Subst.cons (a : Action T) (σ : Subst T) : Subst T := .mk λ n =>
+  match n with
+  | 0 => a
+  | n + 1 => σ.act n
+
+instance : AltCons (Action T) (Subst T) where
+  altCons := Subst.cons
+
+def Ren.append : List Nat -> Ren T -> Ren T
+| .nil, r => r
+| .cons hd tl, r => hd .: append tl r
+
+instance : HAppend (List Nat) (Ren T) (Ren T) where
+  hAppend := Ren.append
+
+instance : HAppend (Std.Rco Nat) (Ren T) (Ren T) where
+  hAppend a := Ren.append a.toList
+
+def Subst.append : List (Action T) -> Subst T -> Subst T
+| .nil, r => r
+| .cons hd tl, r => hd .: append tl r
+
+instance : HAppend (List $ Action T) (Subst T) (Subst T) where
+  hAppend := Subst.append
+
+def Subst.append_ren : List Nat -> Subst T -> Subst T
+| .nil, r => r
+| .cons hd tl, r => re hd .: append_ren tl r
+
+instance : HAppend (List Nat) (Subst T) (Subst T) where
+  hAppend := Subst.append_ren
+
+instance : HAppend (Std.Rco Nat) (Subst T) (Subst T) where
+  hAppend a := Subst.append_ren a.toList
+
+def Ren.compose : Ren T -> Ren T -> Ren T
+| r1, r2 => .mk λ n => r2.act (r1.act n)
+
+instance : AndThen (Ren T) where
+  andThen r f := Ren.compose r (f ())
+
+def RenVec.compose : {V : List (Type u2)} -> RenVec V -> RenVec V -> RenVec V
+| _, nil, _ => nil
+| .cons _ _, cons v1 v1s, cons v2 v2s => (v1 >> v2) .: compose v1s v2s
+
+instance : AndThen (RenVec V) where
+  andThen r f := RenVec.compose r (f ())
+
+def Subst.compose_ren_left : Ren T -> Subst T -> Subst T
+| r, τ => .mk λ n => τ.act (r.act n)
+
+instance : HAndThen (Ren T) (Subst T) (Subst T) where
+  hAndThen r f := Subst.compose_ren_left r (f ())
+
+def SubstVec.compose_ren_left
+  : {V : List (Type u2)} -> RenVec V -> SubstVec V -> SubstVec V
+| [],  _, _ => .nil
+| .cons _ _, .cons v1 v1s, cons v2 v2s => (v1 >> v2) .: compose_ren_left v1s v2s
+
+instance : HAndThen (RenVec V) (SubstVec V) (SubstVec V) where
+  hAndThen r f := SubstVec.compose_ren_left r (f ())
+
+def Subst.compose_ren_right [RenMap T (T::V)] : Subst T -> RenVec (T::V) -> Subst T
+| σ, r => .mk λ n => (σ.act n)⟨r,⟩
+
+instance [RenMap T (T::V)] : HAndThen (Subst T) (RenVec (T::V)) (Subst T) where
+  hAndThen σ f := Subst.compose_ren_right σ (f ())
+
+def SubstVec.compose_ren_right
+  : {V : List (Type u2)} -> [RenMapAll V] -> SubstVec V -> RenVec V -> SubstVec V
+| [], _, _, _ => .nil
+| .cons _ _, _, cons v1 v1s, v@(.cons _ v2s) => (v1 >> v) .: compose_ren_right v1s v2s
+
+instance [RenMapAll V] : HAndThen (SubstVec V) (RenVec V) (SubstVec V) where
+  hAndThen σ f := SubstVec.compose_ren_right σ (f ())
+
+def Subst.compose [SubstMap T (T::V)] : Subst T -> SubstVec (T::V) -> Subst T
+| σ, τ => .mk fun n => (σ.act n)[τ,]
+
+instance [SubstMap T (T::V)] : HAndThen (Subst T) (SubstVec (T::V)) (Subst T) where
+  hAndThen σ f := Subst.compose σ (f ())
+
+def SubstVec.compose
+  : {V : List (Type u2)} -> [SubstMapAll V] ->
+    SubstVec V -> SubstVec V -> SubstVec V
+| [], _, _, _ => .nil
+| .cons _ _, _, cons v1 v1s, v@(cons _ v2s) => (v1 >> v) .: compose v1s v2s
+
+instance [SubstMapAll V] : AndThen (SubstVec V) where
+  andThen σ f := SubstVec.compose σ (f ())
+
+def Ren.lift (r : Ren T) (k : Nat := 1) : Ren T := (0...k) ++ r >> add T k
+
+@[simp]
+def RenVec.lift : {V : List (Type u2)} -> RenVec V -> List Nat -> RenVec V
+| [], _, _ => .nil
+| _::_, cons t ts, [] => t .: ts
+| _::_, cons t ts, k::ks => t.lift k .: ts.lift ks
+
+def Subst.lift' (V : List (Type u2)) [RenMap T (T::V)] (σ : Subst T) (k : Nat := 1) : Subst T :=
+  (0...k) ++ σ >> (.add T k .: RenVec.id V)
+
+def Subst.lift (V : List (Type u2)) [RenMap T (T::V)] (σ : Subst T) (k : Nat := 1) : Subst T := .mk λ n =>
+  if n < k then re n else (σ.act (n - k))⟨.add T k .: .id V,⟩
+
+@[simp]
+def SubstVec.lift : {V : List (Type u2)} -> [RenMapAll V] -> List Nat -> SubstVec V ->  SubstVec V
+| [], _, _, _ => .nil
+| .cons _ _, _, [], cons t ts => t .: ts
+| .cons _ Vs, _, .cons k ks, cons t ts => t.lift Vs k .: ts.lift ks
+
+def Subst.act_list (σ : Subst T) : (ℓ : List Nat) -> List (Action T)
+| [] => []
+| .cons x xs => σ.act x :: act_list σ xs
+
+instance : SubstAction T (List Nat) (List (Action T)) where
+  act := Subst.act_list
+
+def Ren.to (r : Ren T) : Subst T := ⟨λ x => re (r.act x)⟩
+
+def RenVec.to : {V : List (Type u2)} -> (r : RenVec V) -> SubstVec V
+| [], _ => .nil
+| .cons _ _, cons r rs => r.to .: rs.to
 
 end LeanSubst
